compiler/backend/proofs/mod_to_conProofScript.sml
@@ -2771,4 +2771,86 @@ val compile_prog_semantics = Q.store_thm("compile_prog_semantics",
   first_assum(fn th => mp_tac th >> discharge_hyps >- metis_tac[SND]) >>
   strip_tac >> simp[] >> fs[s_rel_cases]);
 
+val prog_to_top_types_def = modSemTheory.prog_to_top_types_def;
+val decs_to_types_def = modSemTheory.decs_to_types_def;
+val prompt_mods_ok_def = modSemTheory.prompt_mods_ok_def;
+
+val alloc_tags_exh_unchanged = Q.store_thm("alloc_tags_exh_unchanged",
+  `∀c b a.
+    ¬MEM (Short t) (MAP (λ(tvs,tn,ctors). mk_id a tn) c) ∧
+    FLOOKUP (get_exh(FST b)) (Short t) = SOME v ⇒
+    FLOOKUP (get_exh(FST(alloc_tags a b c))) (Short t) = SOME v`,
+  Induct >> simp[alloc_tags_def] >>
+  rw[] >> PairCases_on`h` >>
+  simp[alloc_tags_def] >>
+  first_x_assum match_mp_tac >> fs[] >>
+  pop_assum mp_tac >>
+  qid_spec_tac`b` >>
+  Induct_on`h2`>>rw[] >>
+  simp[UNCURRY] >>
+  first_x_assum match_mp_tac >>
+  PairCases_on`b` >>
+  simp[alloc_tag_def] >>
+  every_case_tac >> fs[get_exh_def] >>
+  simp[FLOOKUP_UPDATE]);
+
+val compile_decs_exh_unchanged = Q.store_thm("compile_decs_exh_unchanged",
+  `∀ds a st sta st' ac b.
+   EVERY (λd. case d of Dtype mn _ => mn = SOME x | Dexn mn _ _ => mn = SOME x | _ => T) ds ∧
+   compile_decs sta ds = ((st',ac),b) ∧ st = FST sta ∧
+   FLOOKUP (get_exh st) (Short t) = SOME v
+   ⇒
+   FLOOKUP (get_exh st') (Short t) = SOME v`,
+  Induct >> simp[compile_decs_def] >> rw[] >> fs[] >>
+  every_case_tac >> fs[] >>
+  split_pair_tac >> fs[] >> rveq >>
+  res_tac >> fs[] >>
+  pop_assum kall_tac >>
+  first_x_assum match_mp_tac >- (
+    match_mp_tac alloc_tags_exh_unchanged >>
+    simp[MEM_MAP,UNCURRY,astTheory.mk_id_def] ) >>
+  PairCases_on`sta`>>simp[alloc_tag_def] >>
+  fs[get_exh_def]);
+
+val compile_prompt_exh_unchanged = Q.store_thm("compile_prompt_exh_unchanged",
+  `(∀ds. p = Prompt NONE ds ⇒ ¬MEM t (decs_to_types ds)) ∧
+   (∀mn ds. p = Prompt mn ds ⇒ prompt_mods_ok mn ds) ∧
+   FLOOKUP (get_exh st) (Short t) = SOME v ⇒
+   FLOOKUP (get_exh (FST (compile_prompt st p))) (Short t) = SOME v`,
+  rw[compile_prompt_def] >>
+  BasicProvers.TOP_CASE_TAC >> rw[] >> rw[get_exh_def] >>
+  fs[prompt_mods_ok_def] >>
+  every_case_tac >> fs[] >- (
+    Cases_on`l`>>fs[compile_decs_def] >> rveq >- fs[get_exh_def] >>
+    Cases_on`t'`>>fsrw_tac[ARITH_ss][]>>
+    every_case_tac >> fs[LET_THM] >>
+    split_pair_tac >> fs[] >> rveq >>
+    fs[compile_decs_def] >> rveq >> fs[get_exh_def] >>
+    PairCases_on`st`>>
+    fs[decs_to_types_def,alloc_tag_def,LET_THM] >>
+    rveq >> fs[get_exh_def] >> rw[] >>
+    qmatch_assum_abbrev_tac`alloc_tags a b c = _` >>
+    qispl_then[`c`,`b`,`a`]mp_tac alloc_tags_exh_unchanged >>
+    simp[get_exh_def] >> disch_then match_mp_tac >>
+    simp[Abbr`b`,get_exh_def,MEM_MAP,UNCURRY] >>
+    Cases_on`a`>>simp[astTheory.mk_id_def,FORALL_PROD] >>
+    fs[MEM_MAP,EXISTS_PROD] ) >>
+  imp_res_tac compile_decs_exh_unchanged >> fs[get_exh_def]);
+
+val compile_prog_exh_unchanged = Q.store_thm("compile_prog_exh_unchanged",
+  `∀p st.
+   ¬MEM t (prog_to_top_types p) ∧
+   EVERY (λp. case p of Prompt mn ds => prompt_mods_ok mn ds) p ∧
+   FLOOKUP (get_exh st) (Short t) = SOME v ∧
+   exh' = get_exh (FST (compile_prog st p))
+   ⇒
+   FLOOKUP exh' (Short t) = SOME v`,
+  Induct >> simp[compile_prog_def] >> rw[UNCURRY] >>
+  `¬MEM t (prog_to_top_types p)` by (
+    fs[prog_to_top_types_def] ) >> fs[] >>
+  first_x_assum match_mp_tac >>
+  fs[prog_to_top_types_def] >>
+  match_mp_tac compile_prompt_exh_unchanged >>
+  Cases_on`h`>>fs[]>>rw[]>>fs[]);
+
 val _ = export_theory ();
